O2.3 complete

ivm.v
@@ -28,6 +28,11 @@ Global Unset Printing Primitive Projection Parameters.
 (** printing )-> $){\rightarrow}$ *)
 (** printing >>= $>\!\!>=$ *)
 (** printing not $\neg$ *)
+(** printing <| $\langle|$ *)
+(** printing |> $|\rangle$ *)
+(** printing |>) $|\rangle)$ *)
+(** printing )|>) $)|\rangle)$ *)
+(** printing )|>);; %$)|\rangle)$;;% *)
 
 (** printing fun $\lambda$ #fun# *)
 (** printing nat $\mathbb{N}$ #nat# *)
@@ -45,6 +50,9 @@ Global Unset Printing Primitive Projection Parameters.
 (** printing Bits32 $\mathbb{B}^{32}$ #Bits32# *)
 (** printing Bits64 $\mathbb{B}^{64}$ #Bits64# *)
 
+(** printing m0 $\coqdocvar{m}_0$ *)
+(** printing m1 $\coqdocvar{m}_1$ *)
+(** printing m2 $\coqdocvar{m}_2$ *)
 (** printing s0 $\coqdocvar{s}_0$ *)
 (** printing s1 $\coqdocvar{s}_1$ *)
 (** printing s2 $\coqdocvar{s}_2$ *)
@@ -53,12 +61,13 @@ Global Unset Printing Primitive Projection Parameters.
 (** printing st2 $\coqdocvar{st}_2$ *)
 (** printing x1 $\coqdocvar{x}_1$ *)
 (** printing xn $\coqdocvar{x}_n$ *)
+(** printing IO0 $\coqdocvar{IO}_0$ *)
 (** printing map2 $\coqdocvar{map}_2$ *)
 
 
-(** * Formal virtual machine specification%\label{sec:formal}%
+(** * Formal specification of the iVM abstract machine%\label{sec:formal}%
 
-This section contains a mathematical definition of the virtual machine
+This section contains a mathematical definition of the abstract machine
 used to interpret the contents of this film. It has been formalized in a
 system for formal mathematics called Coq, which is based on higher-order
 type theory. The text below was extracted from the Coq description. It
@@ -116,16 +125,16 @@ Here [A] is an arbitrary type. We use [ [ ] ] and [x :: y] as shortcuts for
 [nil] and [cons x y], respectively.
 
 We will also be using some "dependent" types, such as lists with length
-$n$, known as _vectors_:
+$n$, known as "vectors":
 
 [[
 Definition vector A n := { u : list A | length u = n }.
 ]]
 
 For technical reasons, [vector] is not actually defined like this.
-However, we do have implicit inclusions [vector A n] $↪$ [list A], and
-there is a corresponding vector in [Vector A (length u)] for every [u:
-list A]. *)
+However, we do have implicit inclusions [vector A n] $↪$ [list A] for
+every [n] known as "coercions", and for every [u: list A] there is a
+corresponding element in [vector A (length u)]. *)
 
 (* begin hide *)
 Open Scope bool_scope.
@@ -139,8 +148,8 @@ Coercion to_list: t >-> list.
 (** *** Binary numbers
 
 If we interpret [true] and [false] as 1 and 0, then a list or vector of
-Booleans can be considered a binary in the interval $[0, 2^n)$ where [n =
-length u]. *)
+Booleans can be considered a binary number in the interval $[0, 2^n)$
+where [n = length u]. *)
 
 (* begin hide *)
 Definition boolToNat (x: bool) : nat := if x then 1 else 0.
@@ -152,9 +161,9 @@ Equations fromBits (_: list bool) : nat :=
   fromBits (x :: u) := 2 * fromBits u + x.
 
 (** This definition is formulated using the Equations extension to Coq.
-Observe that the least significant bit comes first. We usually leave
-[fromBits] implicit, using elements of [list bool] and [vector bool n] as if
-they were natural numbers.
+Observe that the least significant bit comes first. Taking [fromBits] as a
+coercion, we will often be using elements of [list bool] and [vector bool n] as
+if they were natural numbers.
 
 Conversely, we can extract the $n$ least significant bits of any integer:
 *)
@@ -165,7 +174,7 @@ Open Scope vector_scope.
 (* end hide *)
 
 Equations toBits (n: nat) (_: Z) : vector bool n :=
-  toBits 0 _ := [] ;
+  toBits O _ := [] ;
   toBits (S n) z := (z mod 2 =? 1) :: toBits n (z / 2).
 (* begin hide *)
 End limit_scope.
@@ -260,8 +269,7 @@ Qed.
 (* end hide *)
 
 (** The most significant bit determines if the [signed u] is negative, and
-[signed u] $\equiv$ [fromBits u] $\pmod{2^n}$ for every [u: vector bool n].
-*)
+[signed u] $\equiv$ [fromBits u] $\pmod{2^n}$ for every [u: vector bool n]. *)
 
 
 (** *** Bytes and words
@@ -300,7 +308,32 @@ Equations toLittleEndian n (_: Z) : vector Bits8 n :=
   toLittleEndian 0 _ := [];
   toLittleEndian (S n) z := (toBits 8 z) :: (toLittleEndian n (z / 256)).
 
-(** Observe that the least significant byte comes first. *)
+(** The least significant byte comes first, and we have the following (not
+entirely commutative) diagram:
+
+%
+\begin{center}
+  \begin{tikzcd}[row sep=normal, column sep=6em]
+    \coqdocvar{list}\;\mathbb{B}
+    \arrow[r, "\coqdocvar{fromBits}"]
+    \arrow[dr, dashed, "\coqdocvar{signed}" sloped] &
+    \mathbb{N}
+    \arrow[d, hook] &
+    \coqdocvar{list}\;\mathbb{B}^8
+    \arrow[l, dashed, swap, "\coqdocvar{fromLittleEndian}"]
+    \\
+    \coqdocvar{vector}\;\mathbb{B}\; n
+    \arrow[u, hook] &
+    \mathbb{Z}
+    \arrow[l, dashed, "\coqdocvar{toBits}\;\coqdocvar{n}"]
+    \arrow[r, dashed, swap, "\coqdocvar{toLittleEndian}\;\coqdocvar{n}"] &
+    \coqdocvar{vector}\;\mathbb{B}^8\; n
+    \arrow[u, hook]
+  \end{tikzcd}
+\end{center}
+%
+
+ *)
 
 (* begin hide *)
 End limit_scope.
@@ -326,28 +359,25 @@ Qed.
 
 (** *** Monads
 
-A monad consist of a generic type [m] and two operations that satisfy
-three axioms. In Coq this can be expressed as a type class: *)
+In this text a "monad" is a structure consisting of one generic type [m:
+Type -> Type] and two operations that satisfy three axioms. We express
+this as a "type class": *)
 
-(* Based on https://github.com/coq/coq/wiki/AUGER_Monad. *)
+(* Loosely based on https://github.com/coq/coq/wiki/AUGER_Monad. *)
 Class Monad (m: Type -> Type): Type :=
 {
-  ret: forall A, A -> m A;
-  bind: forall A, m A -> forall {B}, (A -> m B) -> m B;
+  ret: forall {A}, A -> m A;
+  bind: forall {A}, m A -> forall {B}, (A -> m B) -> m B;
 
-  monad_right: forall A (ma: m A), bind ma (@ret A) = ma;
+  monad_right: forall A (ma: m A), bind ma ret = ma;
   monad_left: forall A (a: A) B (f: A -> m B), bind (ret a) f = f a;
   monad_assoc: forall A (ma: m A) B f C (g: B -> m C),
       bind ma (fun a => bind (f a) g) = bind (bind ma f) g;
 }.
 
-(* begin hide *)
-Notation "ma >>= f" := (bind ma f) (at level 69, left associativity).
-Notation "a ::= ma ; mb" := (bind ma (fun a => mb)) (at level 60, right associativity, only parsing).
-Notation "ma ;; mb" := (bind ma (fun _ => mb)) (at level 60, right associativity).
-(* end hide *)
-
-(** Working with monads, we use the following notation:
+(** Writing the type parameters as [{A}] and [{B}] means that when we
+apply [ret] and [bind], the type arguments should be left implicit.
+Moreover, we use the following notation:
 %
 \begin{center}
 \begin{tabular}{l@{$\qquad$ means $\qquad$}l}
@@ -358,11 +388,15 @@ Notation "ma ;; mb" := (bind ma (fun _ => mb)) (at level 60, right associativity
 %
 \end{tabular}
 \end{center}
-%
-The type arguments ([A] and [B]) are usually implicit. *)
+*)
 
+(* begin hide *)
+Notation "ma >>= f" := (bind ma f) (at level 69, left associativity).
+Notation "a ::= ma ; mb" := (bind ma (fun a => mb)) (at level 60, right associativity, only parsing).
+Notation "ma ;; mb" := (bind ma (fun _ => mb)) (at level 60, right associativity).
+(* end hide *)
 
-(** The simplest monad is the identity monad. *)
+(** The simplest monad is the "identity monad", were [m A = A] for every [A]: *)
 
 (* TODO: Place in module? *)
 Instance IdMonad: Monad id :=
@@ -376,35 +410,63 @@ Proof.
   - reflexivity.
 Defined.
 
+(** We shall often say that a function [Type -> Type] is a monad if the
+rest of the monad structure is clear from the context. *)
 
-(** *** Monad transformers *)
 
-Class Morphism {m1} `{Monad m1} {m2} `{Monad m2} (F: forall {A}, m1 A -> m2 A) :=
+(** *** Monad transformers
+
+A "morphism" between monads is a structure preserving family of functions
+[m0 A -> m1 A] : *)
+
+Class Morphism m0 `{Monad m0} m1 `{Monad m1} (F: forall {A}, m0 A -> m1 A) :=
 {
   morph_ret: forall A (x: A), F (ret x) = ret x;
-  morph_bind: forall A (ma: m1 A) B (f: A -> m1 B),
+  morph_bind: forall A (ma: m0 A) B (f: A -> m0 B),
       F (ma >>= f) = (F ma) >>= (fun x => F (f x));
 }.
+
+Arguments Morphism: clear implicits.
+Arguments Morphism _ {_} _ {_} _.
+
+(** Here [`{Monad m0}] means that that [m0: Type -> Type] must have a
+(usually implicit) monad structure, similarly for [m1]. A "monad
+transformer" constructs a new monad from an existing monad [m] such that
+there is a morphism from [m] to the new monad: *)
 
 Class Transformer (t: forall (m: Type -> Type) `{Monad m}, Type -> Type): Type :=
 {
   transformer_monad: forall m `{Monad m}, Monad (t m);
-  lift: forall {m} `{Monad m} {A}, m A -> (t m) A;
-  lift_morphism: forall {m} `{Monad m}, Morphism (@lift _ _);
+  lift: forall {m} `{Monad m} A, m A -> (t m) A;
+  lift_morphism: forall {m} `{Monad m}, Morphism _ _ lift;
 }.
+
+(* begin hide*)
 
 Existing Instance transformer_monad.
 Existing Instance lift_morphism.
 
-Definition Opt m `{mo:Monad m} A := m (option A).
+(* end hide *)
+
+(** We get a simple transformer by composing [m] with [option] (as defined
+above): *)
+
+Definition Opt m `{Monad m} A := m (option A).
+
+(* begin hide *)
+
+Arguments Opt: clear implicits.
+Arguments Opt _ {_}.
+
+(* end hide *)
 
 Instance OptionTransformer: Transformer Opt :=
 {
-  transformer_monad m mo :=
+  transformer_monad m _ :=
     {|
-      ret A x := ret (Some x);
-      bind A ma B f := bind (A:=option A) ma
-                            (fun a => match a with None => ret None | Some x => f x end);
+      ret _ x := ret (Some x);
+      bind _ ma _ f := a ::= (ma: m _);
+                       match a with None => ret None | Some x => f x end;
     |};
   lift _ _ _ ma := x ::= ma; ret (Some x);
 }.
@@ -441,15 +503,17 @@ Proof.
       reflexivity.
 Defined.
 
-(* TODO: Explain *)
+(** Here we define [ret] and [bind] in terms of the corresponding
+operations of [m]. The axioms are easy to verify. Monads of the form [Opt
+m] can represent computations that may stop before producing a value: *)
 
-Definition stop' {m} `{mo: Monad m} {A}: Opt A := ret None.
+Definition stop' {m} `{Monad m} {A}: Opt m A := ret None.
 
 (** Observe that [stop' >>= f = stop'] for every [f]. *)
 
 (* begin hide *)
 
-Lemma stop_bind : forall m `(mo: Monad m) A B (f: A -> Opt B), stop' >>= f = stop'.
+Lemma stop_bind : forall m `(M: Monad m) A B (f: A -> Opt m B), stop' >>= f = stop'.
 Proof.
   intros.
   unfold stop'.
@@ -458,8 +522,8 @@ Proof.
   reflexivity.
 Qed.
 
-Instance opt_morphism: forall m1 `(mo1: Monad m1) m2 `(mo2: Monad m2) (F: forall A, m1 A -> m2 A) `(mor: @Morphism m1 _ m2 _ F),
-    @Morphism (@Opt m1 _) _ (@Opt m2 _) _ (fun A => F (option A)).
+Instance opt_morphism: forall m0 `(Monad m0) m1 `(Monad m1) (F: forall A, m0 A -> m1 A) `(Morphism m0 m1 F),
+    Morphism (Opt m0) (Opt m1) (fun A => F (option A)).
 Proof.
   intros.
   split.
@@ -477,6 +541,14 @@ Qed.
 
 (* end hide *)
 
+
+(** *** State monad transformer
+
+As discovered by Eugenio Moggi in 1989, monads can be used to represent
+computations with side-effects such as input and output. In particular, we
+can define a transformer which extends and existing monad with the ability
+to access and modify a value referred to as the "current state": *)
+
 (* begin hide *)
 Section limit_scope.
 Open Scope type_scope.
@@ -485,17 +557,22 @@ Open Scope type_scope.
 Definition ST S m `{Monad m} A := S -> m (A * S).
 
 (* begin hide *)
+
 End limit_scope.
+
+Arguments ST: clear implicits.
+Arguments ST _ _ {_} _.
+
 (* end hide *)
 
 Instance StateTransformer S: Transformer (ST S) :=
 {
-  transformer_monad m mo :=
+  transformer_monad m _ :=
     {|
-      ret A x s := ret (x, s);
-      bind A ma B f s := bind (ma s) (fun p => f (fst p) (snd p));
+      ret _ x := fun s => ret (x, s);
+      bind _ ma _ f := fun s => p ::= ma s; f (fst p) (snd p);
     |};
-  lift _ _ _ ma s := bind ma (fun x => ret (x, s));
+  lift _ _ _ ma := fun s => x ::= ma; ret (x, s);
 }.
 Proof. (* TODO: The proofs are virtually identical to those of the option transformer. *)
   - intros.
@@ -537,19 +614,15 @@ Proof. (* TODO: The proofs are virtually identical to those of the option transf
       reflexivity.
 Defined.
 
-(** TODO: Explain state monad transformer *)
+(** In other words, [ST S] is a monad transformer for every type [S]. We
+shall be especially interested in monads of the form [Opt (ST S m)] where
+the elements represent "computations": *)
 
-Section opt_st_facts.
+Section opt_st_section.
 
-  Context {m} `{mo: Monad m} {S: Type}.
+  Context {m} `{Monad m} {S: Type}.
 
-  Let C := @Opt (@ST S m _) _.
-
-  Proposition ST_stop: forall A (s: S),
-      @stop' (@ST S m _) _ A s = ret (None, s).
-  Proof.
-    reflexivity.
-  Qed.
+  Let C := Opt (ST S m).
 
   Definition tryGet' {A} (f: S -> option A) : C A :=
     fun s => ret (f s, s).
@@ -557,25 +630,27 @@ Section opt_st_facts.
   Definition get' {A} (f: S -> A) : C A :=
     fun s => ret (Some (f s), s).
 
-  Definition updateState' (f: S -> S): C unit :=
+  Definition update' (f: S -> S): C unit :=
     fun s => ret (Some tt, f s).
 
-  (** We use the convention that computations (and functions returning
+  (** These definitions were simplified by placing them inside a "section"
+      with a list of shared [Context] parameters and a local abbreviation,
+      [C]. In this text computations (and functions returning
       computations) have names ending with an apostrophe. For this reason
       we also define: *)
 
   Definition return' {A} (x: A) : C A := ret x.
 
-End opt_st_facts.
+End opt_st_section.
 
 
-(** ** Core machine state
+(** ** Generic abstract machine%\label{sec:generic}%
 
-As discovered by Eugenio Moggi in 1989, monads can be used to represent
-computations with side-effects such as input and output. Below we shall
-define a virtual machine in terms of a partial computational monad, but
-first we define types representing the state of the machine at a given
-moment. *)
+We have split specification of the machine in three parts. In
+section%~\ref{sec:io}% we specify the I/O operations in terms of a
+separate monad, [IO], whereas in the current section we describe the parts
+of the machine that are independent of the I/O operations. Finally, we put
+the pieces together in section%\ref{sec:integration}%. *)
 
 (* begin hide *)
 
@@ -615,7 +690,16 @@ Module Instructions.
   Notation "'XOR'" := 43.
   Notation "'POW2'" := 44.
 End Instructions.
+
 (* end hide *)
+
+(** The current state of the generic virtual machine has three components:
+a program counter ([PC]), a stack pointer ([SP]), and the memory contents.
+The memory is a collection of memory cells. Each cell has a unique address
+of type [Bits64] and stores one byte of data. In practice, the addresses
+of the memory cells will form a subset $[0,\coqdocvar{memorySize})$ for
+some $\coqdocvar{memorySize}\leq 2^{64}$, see [initialCoreState] below.
+*)
 
 Record CoreState :=
   mkCoreState {
@@ -625,8 +709,8 @@ Record CoreState :=
     }.
 
 (** A record is an inductive type with a single constructor
-([mkCoreState]), where we get projections for free. For example, if [s:
-CoreState], then [PC s: Bits64]. *)
+([mkCoreState]), where we get projections for free. For example, [PC s :
+Bits64] for every [s : CoreState]. *)
 
 (* begin hide *)
 
@@ -648,29 +732,37 @@ Definition initialCoreState
     memory a := nth a (map Some mem) None
   |}.
 
-(** In other words, before the virtual machine is started, the available
-memory should be initialized to 0 except for a "program" and a "argument",
-both sequenced of bytes. Moreover, the (64-bit) length of the argument is
-stored between the program and the argument, the program counter is
-initialized to 0 and the stack pointer to the first address after the
-available memory. *)
+(** In other words, before the machine is started, the available memory
+will be initialized to 0, except for a "program" and an "argument", both
+sequenced of bytes. Also, the length of the argument is stored in 64 bits
+between the program and the argument, the program counter is set to 0, and
+the stack pointer is set to the first address after the available memory.
+*)
 
 
-Section Core.
+Section generic_machine_section.
 
-  (* IO monad without stopping. *)
-  Context m `{mo: Monad m}.
-  Let IO := @Opt m mo.
+  (** We assume an I/O monad of form [Opt m] (to be defined later). *)
 
-  Definition Comp := @Opt (@ST CoreState m mo) _.
+  Context m `{Monad m}.
 
-  Definition fromIO A : IO A -> Comp A := lift (A := option A).
+  Let IO := Opt m.
 
-  Instance fromIO_morphism: @Morphism IO _ Comp _ fromIO.
+  Definition Comp := Opt (ST CoreState m).
+
+  Definition fromIO {A} : IO A -> Comp A := lift (option A).
+
+  (* begin hide *)
+  Arguments fromIO [A].
+  (* end hide *)
+
+  Instance fromIO_morphism: Morphism IO Comp fromIO.
   Proof.
     (* intros. apply opt_morphism, lift_morphism. *)
     typeclasses eauto.
   Qed.
+
+  (** Also observe that [fromIO stop' = stop']. *)
 
   (* begin hide *)
 
@@ -683,9 +775,9 @@ Section Core.
   (* end hide *)
 
 
-  (** *** Memory access *)
+  (** *** Memory access
 
-  (** The virtual machine uses 64-bit memory addresses. *)
+  The machine stops if it is asked to access an unavailable memory address: *)
 
   Definition loadByte' (a: Z) : Comp Bits8 :=
     mem ::= get' memory;
@@ -714,12 +806,9 @@ Section Core.
     bytes ::= loadBytes' n a;
     return' (fromLittleEndian bytes).
 
-  (** That is, [load' n a s0 = (Some x, s1)] if [s0 = s1] and the [n] bytes
-  starting at [a] represent the natural number [x] $<2^n$. If not all the
-  addresses [a], ..., [a+n-1] are available, the machine stops.
-
-  [storeByte'] tries to change the value at a memory address, but stops if
-  the address is not available: *)
+  (** That is, [load' n a s0 = (Some x, s1)] if [s0 = s1] and the [n]
+  bytes at addresses [a], ..., [a+n-1] represent the natural number [x]
+  $<2^n$. [storeByte'] also stops if the address is not available: *)
 
   Definition storeByte' (a: Z) (value: Bits8) : Comp unit :=
     mem ::= get' memory;
@@ -727,11 +816,11 @@ Section Core.
     match mem u with
     | None => stop'
     | _ => let newMem (v: Bits64) := if v =? u then Some value else mem v in
-          updateState' (fun s => s <| memory := newMem |>)
+          update' (fun s => s<|memory := newMem|>)
     end.
 
-  (** Here [s <| memory := newMem |>] denotes a record which is identical
-  to [s] except that the field [memory] has been changed to [newMem]. *)
+  (** Here [s<|memory := newMem|>] is identical to [s], except that the
+  field [memory] has been changed to [newMem]. *)
 
   Equations storeBytes' (_: Z) (_: list Bits8) : Comp unit :=
     storeBytes' _ [] := return' tt;
@@ -743,18 +832,29 @@ Section Core.
     storeBytes' start (toLittleEndian n value).
 
 
-  (** *** Stack and program counter *)
+  (** *** Program counter *)
 
   Definition setPC' (az: Z): Comp unit :=
-    updateState' (fun s => s <| PC := toBits 64 az |>).
-
-  Definition setSP' (az: Z): Comp unit :=
-    updateState' (fun s => s <| SP := toBits 64 az |>).
+    update' (fun s => s<|PC := toBits 64 az|>).
 
   Definition next' (n: nat) : Comp nat :=
     a ::= get' PC;
     setPC' (a + n);;
     load' n a.
+
+  (** In other words, [next' n] loads the next [n] bytes and advances [PC]
+  accordingly. *)
+
+
+  (** *** Stack
+
+  A stack is a LIFO (last in, first out) queue. The elements on our stack
+  are 64 bits long, and [SP] points to the next element that can be
+  popped. The stack grows "downwards" in the sense that [SP] is decreased
+  when new elements are pushed. *)
+
+  Definition setSP' (az: Z): Comp unit :=
+    update' (fun s => s<|SP := toBits 64 az|>).
 
   Definition pop': Comp Bits64 :=
     a ::= get' SP;
@@ -771,9 +871,6 @@ Section Core.
     popN' 0 := return' [];
     popN' (S n) := u ::= popN' n; x ::= pop'; return' (x :: u).
 
-  (** Observe that the result from [popN'] comes in the order was pushed.
-  *)
-
   (* begin hide *)
   End limit_scope.
   (* end hide *)
@@ -788,8 +885,17 @@ Section Core.
     pushList' [] := return' tt;
     pushList' (x :: u) := push' x;; pushList' u.
 
+  (** Since [popN'] returns elements in the order they were pushed, it is
+  essentially a left inverse to [pushList']. *)
 
-  (** *** Abstract I/O *)
+
+  (** *** Generic I/O interface
+
+  In the generic machine an I/O operation is simply an element [io: vector
+  Bits64 n -> IO (list Bits64)] for some [n]. When a corresponding
+  operation is encountered, the machine will pop [n] elements from the
+  stack, execute [io] on these elements and place the push the result onto
+  the stack. *)
 
   Record IO_operation :=
     mkIO_operation {
@@ -805,14 +911,15 @@ Section Core.
   Context (IO_operations: list IO_operation).
 
   Definition ioStep' (n: nat) : Comp unit :=
-    if n <? 128
-    then stop'
-    else nth (n - 128) (map from_IO_operation IO_operations) stop'.
+    nth (255 - n) (map from_IO_operation IO_operations) stop'.
+
+  (** In other words, we assume a list of I/O operations that will be
+  mapped to "opcodes" 255, 254, ...*)
 
 
-  (** ** Single execution step
+  (** *** Single execution step
 
-  The virtual machine has the following core "opcodes":
+  The other opcodes of the machine are as follows:
 
   %
   \newcommand\col[1]{\begin{tabular}[t]{rl}#1\end{tabular}}
@@ -852,6 +959,8 @@ Section Core.
   34 & \coqdocvar{DIV}\\
   35 & \coqdocvar{REM}\\
   36 & \coqdocvar{LT}\\
+  }
+  \col{
   40 & \coqdocvar{AND}\\
   41 & \coqdocvar{OR}\\
   42 & \coqdocvar{NOT}\\
@@ -869,8 +978,8 @@ Section Core.
   Let map2 (f: bool->bool->bool) (u: Bits64) (v: Bits64) : Bits64 := Vector.map2 f u v.
   (* end hide *)
 
-  (** %\vspace{1ex}% Now we can define what it means for our virtual machine
-  to perform one execution step. *)
+  (** %\vspace{1ex}% Now we can define what it means for our abstract machine
+  to perform one execution step: *)
 
   Definition oneStep' : Comp unit :=
     opcode ::= next' 1;
@@ -881,8 +990,8 @@ Section Core.
     | JUMP => pop' >>= setPC'
     | JUMP_ZERO =>
         offset ::= next' 1;
-        v ::= pop';
-        if v =? 0
+        x ::= pop';
+        if x =? 0
         then pc ::= get' PC;
              setPC' (pc + (signed (toBits 8 offset)))
         else return' tt
@@ -895,18 +1004,18 @@ Section Core.
     | PUSH2 => next' 2 >>= push'
     | PUSH4 => next' 4 >>= push'
     | PUSH8 => next' 8 >>= push'
-    | SIGX1 => v ::= pop'; push' (signed (toBits 8 v))
-    | SIGX2 => v ::= pop'; push' (signed (toBits 16 v))
-    | SIGX4 => v ::= pop'; push' (signed (toBits 32 v))
+    | SIGX1 => x ::= pop'; push' (signed (toBits 8 x))
+    | SIGX2 => x ::= pop'; push' (signed (toBits 16 x))
+    | SIGX4 => x ::= pop'; push' (signed (toBits 32 x))
 
     | LOAD1 => pop' >>= load' 1 >>= push'
     | LOAD2 => pop' >>= load' 2 >>= push'
     | LOAD4 => pop' >>= load' 4 >>= push'
     | LOAD8 => pop' >>= load' 8 >>= push'
-    | STORE1 => a ::= pop'; v ::= pop'; store' 1 a v
-    | STORE2 => a ::= pop'; v ::= pop'; store' 2 a v
-    | STORE4 => a ::= pop'; v ::= pop'; store' 4 a v
-    | STORE8 => a ::= pop'; v ::= pop'; store' 8 a v
+    | STORE1 => a ::= pop'; x ::= pop'; store' 1 a x
+    | STORE2 => a ::= pop'; x ::= pop'; store' 2 a x
+    | STORE4 => a ::= pop'; x ::= pop'; store' 4 a x
+    | STORE8 => a ::= pop'; x ::= pop'; store' 8 a x
 
     | ADD => x ::= pop'; y ::= pop'; push' (x + y)
     | MULT => x ::= pop'; y ::= pop'; push' (x * y)
@@ -969,10 +1078,10 @@ Section Core.
   Lemma nSteps_stop: forall (init: Comp unit) n,
       init;; nSteps' n;; stop' = init;; nSteps' n -> init;; nSteps' (S n) = init;; nSteps' n.
   Proof.
-    intros init n H.
+    intros init n HH.
     rewrite nSteps_succ.
     rewrite monad_assoc.
-    rewrite <- H.
+    rewrite <- HH.
     repeat rewrite <- monad_assoc.
     rewrite stop_bind.
     reflexivity.
@@ -981,7 +1090,7 @@ Section Core.
   Lemma nSteps_stop_k: forall (init: Comp unit) n k,
       init;; nSteps' n;; stop' = init;; nSteps' n -> init;; nSteps' (k + n) = init;; nSteps' n.
   Proof.
-    intros init n k H.
+    intros init n k HH.
     induction k as [|k IH].
     - reflexivity.
     - rewrite plus_Sn_m.
@@ -990,35 +1099,42 @@ Section Core.
       rewrite monad_assoc.
       rewrite IH.
       rewrite <- monad_assoc.
-      exact H.
+      exact HH.
   Qed.
 
   (* end hide *)
 
-End Core.
+End generic_machine_section.
 
 
-(** ** Input and output *)
+(** ** Actual input and output%\label{sec:io}%
 
-(** *** IO state
+In this section we shall define the I/O operations in terms of a
+corresponding monad. For simplicity, we will again use a monad of the form
+[Opt (ST S m)]; but whereas a concrete implementation of the iVM machine
+would typically reflect [CoreState] in its program state, the I/O state
+might be distributed across the system as a whole. For instance,
+[readFrame'] (defined below) might trigger a scan the next frame of the
+film roll on the fly. It is not necessary to perform a complete scan
+before starting the machine.
 
-An image is a two-dimensional matrix of pixels, counting from left to
-right and from top to bottom. *)
+*** Bitmap images
+
+The I/O state has several components. First, an image is a two-dimensional
+matrix of square pixels, counting from left to right and from top to
+bottom. *)
 
 Record Image (C: Type) :=
   mkImage {
       iWidth: Bits16;
       iHeight: Bits16;
       iPixel: nat -> nat -> option C;
-      iDef: forall x y, iPixel x y <> None <-> x < iWidth /\ y < iHeight;
+      iDefined: forall x y, iPixel x y <> None <-> x < iWidth /\ y < iHeight;
     }.
 
-(** A record is an inductive type with a single constructor ([mkImage]),
-where we get projections for free. For example, if [im: Image Bits8], then
-[iWidth im: Bits16]. The arguments to [iWidth] and [iHeight] are implicit
-in the type of iDef. The type [C] represents the color of a single pixel.
-
-The simplest image consists of [0 * 0] pixels:
+(** Here [C] represents the color of a single pixel. The arguments to
+[iWidth] and [iHeight] (of type [Image C]) are implicit in the type of
+[iDefined]. The simplest image consists of [0 * 0] pixels:
 
 [[
 Definition noImage {C} : Image C :=
@@ -1026,7 +1142,7 @@ Definition noImage {C} : Image C :=
      iWidth := toBits 16 0;
      iHeight := toBits 16 0;
      iPixel := fun _ _ => None;
-     iDef := _;
+     iDefined := _;
   |}.
 ]]
 *)
@@ -1038,7 +1154,7 @@ Definition noImage {C} : Image C.
              iWidth := toBits 16 0;
              iHeight := toBits 16 0;
              iPixel := fun _ _ => None;
-             iDef := _;
+             iDefined := _;
            |}).
   unfold fromBits16.
   rewrite zeroBits_zero.
@@ -1051,9 +1167,8 @@ Defined.
 
 (* end hide *)
 
-(** [Gray] represents the gray scale of the input images (where 0 is
-black), whereas [Color] represents the ACES2065-1 encoded colors of the
-output images: *)
+(** [Gray] represents the gray scale of the input images, and [Color] the
+colors of the output images: *)
 
 (* begin hide *)
 
@@ -1063,20 +1178,20 @@ Open Scope type_scope.
 (* end hide *)
 
 Definition Gray := Bits8.
-Definition Color := Bits16 * Bits16 * Bits16.
+Definition Color := Bits64 * Bits64 * Bits64.
 
-(* begin hide *)
+(** *** Sound and text
 
-(** The [Sound] type represents a clip of stereo sound in LPCM encoding.
-Both channels have the same sample rate, and each pair of 16-bit words
-$[(\coqdocvar{left}, \coqdocvar{right})]$ contains one sample for each
-channel. For convenience, [sSamples] contains samples in reverse order. *)
+[Sound] represents a clip of stereo sound. Both channels have the same
+sample rate, and each pair of 16-bit words $(\coqdocvar{left},
+\coqdocvar{right})$ contains one sample for each channel. For convenience,
+[sSamples] lists the samples in reverse order. *)
 
 Record Sound :=
   mkSound {
       sRate: Bits32;
       sSamples: list (Bits16 * Bits16);
-      sDef: 0 = sRate -> sSamples = [];
+      sDefined: 0 = sRate -> sSamples = [];
     }.
 
 (**
@@ -1091,9 +1206,9 @@ Definition emptySound (rate: Bits32) : Sound :=
 
 (* begin hide *)
 
-Definition emptySound (rate: Bits32) : Sound.
+Definition emptySound (rate: nat) : Sound.
   refine ({|
-             sRate := rate;
+             sRate := (toBits 32 rate);
              sSamples := [];
            |}).
   trivial.
@@ -1101,21 +1216,24 @@ Defined.
 
 (* end hide *)
 
-Definition noSound := emptySound (toBits 32 0).
+Definition noSound := emptySound 0.
 
 (** Textual output from the machine uses the encoding UTF-32. Again, we
 use reverse ordering. *)
 
 Definition OutputText := list Bits32.
 
-Definition Output := (Image Color) * Sound * OutputText.
+Definition OneOutput := (Image Color) * Sound * OutputText.
 
-(** The complete I/O state of our machine can now be defined as: *)
+
+(** *** The I/O monad
+
+The complete I/O state of our machine can now be defined as: *)
 
 Record IoState :=
   mkIoState {
       input: list (Image Gray);
-      output: list Output;
+      output: list OneOutput;
     }.
 
 (* begin hide *)
@@ -1136,19 +1254,21 @@ Definition initialIoState (inputList: list (Image Gray)) :=
     output := [(noImage, noSound, [])]
   |}.
 
-(** As the machine executes [input] will consist of the input frame
-currently being processed and the rest of the film, whereas whereas
-[output] will consist of the
+(** As the machine executes, [input] will decrease in size, whereas
+[output] will increase. The first element in each list represents the
+frame currently being processed/produced. In other words, we use a reverse
+ordering for [output] as well. The I/O monad is based on the identity
+monad: *)
 
-increase. The
+Definition IO0 := ST IoState id.
 
-r *)
+Definition IO := Opt IO0.
 
-Definition IO0 := @ST IoState id _.
-Definition IO := @Opt IO0 _.
+
+(** *** Input operations *)
 
 Definition readFrame' : IO (Bits16 * Bits16) :=
-  updateState' (fun s => s <| input := tail (input s) |>);;
+  update' (fun s => s<|input := tail (input s)|>);;
   i ::= get' input;
   return' (match i with
            | frame :: _ => (iWidth frame, iHeight frame)
@@ -1168,21 +1288,10 @@ Definition readPixel' (x y: nat) : IO Bits8 :=
     end
   end.
 
-Definition defaultColor : Color := (toBits 16 0, toBits 16 0, toBits 16 0).
 
-(**
-[[
-Definition blank (width: Bits16) (height: Bits16): Image Color :=
-  {|
-    iWidth := width;
-    iHeight := height;
-    iPixel x y := if (x <? width) && (y <? height) then Some defaultColor else None;
-    iDef := _;
-  |}.
-]]
+(** *** Output operations *)
 
-Here %\:%[p && q = if p then q else false]. *)
-
+Definition defaultColor: Color := let z := toBits 64 0 in (z, z, z).
 (* begin hide *)
 
 Ltac derive name term :=
@@ -1204,7 +1313,7 @@ Definition blank (width: Bits16) (height: Bits16): Image Color.
         iWidth := width;
         iHeight := height;
         iPixel x y := if (x <? width) && (y <? height) then Some defaultColor else None;
-        iDef := _;
+        iDefined := _;
       |}
     ).
   intros x y.
@@ -1230,27 +1339,38 @@ Definition blank (width: Bits16) (height: Bits16): Image Color.
 Defined.
 
 (* end hide *)
+(**
+[[
+Definition blank (width: Bits16) (height: Bits16): Image Color :=
+  {|
+    iWidth := width;
+    iHeight := height;
+    iPixel x y := if (x <? width) && (y <? height) then Some defaultColor else None;
+    iDefined := _;
+  |}.
+]]
 
+Here %\:%[p && q = if p then q else false]. *)
 
 Definition newFrame' (width height rate: nat) : IO unit :=
-  let o := (blank (toBits 16 width) (toBits 16 height), emptySound (toBits 32 rate), []) in
-  updateState' (fun s => s <| output := o :: output s |>).
+  let o := (blank (toBits 16 width) (toBits 16 height), emptySound rate, []) in
+  update' (fun s => s<|output := o :: output s|>).
 
-Definition getCurrentOutput' : IO Output :=
+Definition getCurrentOutput' : IO OneOutput :=
   oList ::= get' output;
   match oList with
   | o :: _ => return' o
   | [] => stop'
   end.
 
-(** In practice, [getCurrentOutput'] will not halt since we start the
-machine with a non-empty output list, see [initialIoState] above. *)
+(** In practice, [getCurrentOutput'] will not stop since we start the
+machine with a non-empty output list. *)
 
-Definition replaceOutput o s : IoState := s <| output := o :: tail (output s) |>.
+Definition replaceOutput o s : IoState := s<|output := o :: tail (output s)|>.
 
 (**
 [[
-Definition trySetPixel {C} (image: Image C) (x y: nat) (c: C): option (Image C) :=
+Definition trySetPixel (image: Image Color) (x y: nat) (c: Color): option (Image Color) :=
   if (x <? iWidth image) && (y <? iHeight image)
   then let p xx yy := if (xx =? x) && (yy =? y)
                      then Some c
@@ -1262,7 +1382,7 @@ Definition trySetPixel {C} (image: Image C) (x y: nat) (c: C): option (Image C) 
 
 (* begin hide *)
 
-Definition trySetPixel {C} (image: Image C) (x y: nat) (c: C): option (Image C).
+Definition trySetPixel (image: Image Color) (x y: nat) (c: Color): option (Image Color).
   refine (let newPix xx yy := if (xx =? x) && (yy =? y) then Some c else iPixel image xx yy in
           if Sumbool.sumbool_of_bool ((x <? iWidth image) && (y <? iHeight image))
           then Some
@@ -1270,7 +1390,7 @@ Definition trySetPixel {C} (image: Image C) (x y: nat) (c: C): option (Image C).
                    iWidth := iWidth image;
                    iHeight := iHeight image;
                    iPixel := newPix;
-                   iDef := _
+                   iDefined := _
                  |}
           else None).
   subst newPix.
@@ -1290,9 +1410,9 @@ Definition trySetPixel {C} (image: Image C) (x y: nat) (c: C): option (Image C).
       derive H (proj1 (reflect_it (Nat.eqb_spec _ _)) H);
       subst;
       exact e.
-  - apply (iDef image).
+  - apply (iDefined image).
   - discriminate.
-  - apply (iDef image).
+  - apply (iDefined image).
 Defined.
 
 (* end hide *)
@@ -1300,9 +1420,9 @@ Defined.
 Definition setPixel' (x y r g b : nat) : IO unit :=
   o ::= getCurrentOutput';
   match o with (image, sound, text) =>
-    match trySetPixel image x y (toBits 16 r, toBits 16 g, toBits 16 b) with
+    match trySetPixel image x y (toBits 64 r, toBits 64 g, toBits 64 b) with
     | None => stop'
-    | Some newImage => updateState' (replaceOutput (newImage, sound, text))
+    | Some newImage => update' (replaceOutput (newImage, sound, text))
     end
   end.
 
@@ -1312,10 +1432,10 @@ Definition setPixel' (x y r g b : nat) : IO unit :=
 Definition addSample' (l r : nat) : Comp unit :=
   o ::= getCurrentOutput';
   match o with (image, sound, text) =>
-    if sRate sound ?= 0
+    if sRate sound =? 0
     then stop'
     else let ns := sound <| sSamples := (toBits 16 l, toBits 16 r) :: sSamples sound |> in
-         updateState' (replaceOutput (image, ns, text))
+         update' (replaceOutput (image, ns, text))
   end.
 ]]
 *)
@@ -1326,7 +1446,7 @@ Definition addSample (s: Sound) (H: 0 <> sRate s) (l: Bits16) (r: Bits16) :=
   {|
     sRate := sRate s;
     sSamples := (l, r) :: (sSamples s);
-    sDef := fun H0 => False_ind _ (H H0);
+    sDefined := fun H0 => False_ind _ (H H0);
   |}.
 
 Definition addSample' (l r : nat) : IO unit :=
@@ -1336,7 +1456,7 @@ Definition addSample' (l r : nat) : IO unit :=
     | left _ => stop'
     | right H =>
       let newSound := addSample sound (beq_nat_false _ _ H) (toBits 16 l) (toBits 16 r) in
-      updateState' (replaceOutput (image, newSound, text))
+      update' (replaceOutput (image, newSound, text))
     end
   end.
 
@@ -1345,18 +1465,20 @@ Definition addSample' (l r : nat) : IO unit :=
 Definition putChar' (c: nat) : IO unit :=
   o ::= getCurrentOutput';
   match o with (image, sound, text) =>
-    updateState' (replaceOutput (image, sound, (toBits 32 c) :: text))
+    update' (replaceOutput (image, sound, (toBits 32 c) :: text))
   end.
 
 
-(** *** Putting the pieces together
+(** *** List of I/O operations
 
-
-[nFun n A B = A -> A -> ... -> B] *)
+The generic machine defined in section%~\ref{sec:generic}% expects I/O
+operations of a certain form. *)
 
 Equations nFun (n: nat) (A B: Type): Type :=
   nFun O _ B := B;
   nFun (S n) A B := A -> (nFun n A B).
+
+(** In other words, [nFun n A B = ]$\underbrace{A\rightarrow A\rightarrow ...}_n$[ -> B]. *)
 
 (* begin hide *)
 Open Scope vector_scope.
@@ -1383,21 +1505,25 @@ Definition IO_operations :=
     io_operation 1 (fun c => putChar' c;; return' [])
   ].
 
-(* begin hide *)
 
+
+(** ** Integration%\label{sec:integration}%
+
+Putting everthing together, we can say what it means to run the machine
+from start to finish. *)
+
+(* begin hide *)
 (* Why is this needed?*)
 Instance CompMonad: Monad (Comp (m:=IO0)).
 Proof.
   unfold Comp.
   typeclasses eauto.
 Defined.
-
 (* end hide *)
 
-
 Lemma characterize_stopped: forall (c: Comp (m:=IO0) unit) (cs: CoreState) (ios: IoState),
-    let init := updateState' (fun _ => cs);; fromIO _ (updateState' (fun _ => ios)) in
-    init;; c;; stop' = init;; c <-> fst (fst (c cs ios)) = None.
+    let init := update' (fun _ => cs);; fromIO (update' (fun _ => ios)) in
+    init;; c;; stop' = init;; c  <->  fst (fst (c cs ios)) = None.
 Proof. (* TODO: Improve proof *)
   intros.
   split; intro H.
@@ -1419,8 +1545,16 @@ Proof. (* TODO: Improve proof *)
     reflexivity.
 Qed.
 
+(* begin hide *)
+Section limit_scope.
+Open Scope type_scope.
+(* end hide *)
 
-Definition State: Type := CoreState * IoState.
+Definition State := CoreState * IoState.
+
+(* begin hide *)
+End limit_scope.
+(* end hide *)
 
 Definition finalState
            program argument (free: nat) inputList
@@ -1448,7 +1582,7 @@ Proof. (* TODO: simplify *)
     destruct s1.
     destruct s2.
     f_equal; assumption.
-  - set (init := updateState' (fun _ => cs);; fromIO _ (updateState' (fun _ => ios))).
+  - set (init := update' (fun _ => cs);; fromIO (update' (fun _ => ios))).
     assert (init;; g n1;; stop' = init;; g n1) as Hs1; [apply characterize_stopped; rewrite H1; reflexivity|].
     assert (init;; g n2;; stop' = init;; g n2) as Hs2; [apply characterize_stopped; rewrite H2; reflexivity|].
 
